qcp/ast/VC/thm_apply_proof_auto.v
@@ -16,9 +16,16 @@ Local Open Scope sets.
 Local Open Scope string.
 Local Open Scope list.
 Import naive_C_Rules.
+Require Import sll_merge_rel_lib.
+Local Open Scope stmonad.
+From AUXLib Require Import int_auto Axioms Feq Idents List_lemma VMap relations.
 From SimpleC.EE Require Import ast_lib.
 From SimpleC.EE Require Import malloc.
 From SimpleC.EE Require Import sll_tmpl.
+Import naive_C_Rules.
+Require Import sll_merge_rel_lib.
+Local Open Scope stmonad.
+From AUXLib Require Import int_auto Axioms Feq Idents List_lemma VMap relations.
 Local Open Scope sac.
 
 Lemma proof_of_sub_thm_safety_wit_1 : sub_thm_safety_wit_1.
@@ -114,21 +121,6 @@ Proof. Admitted.
 Lemma proof_of_check_list_gen_safety_wit_4 : check_list_gen_safety_wit_4.
 Proof. Admitted. 
 
-Lemma proof_of_check_list_gen_safety_wit_5 : check_list_gen_safety_wit_5.
-Proof. Admitted. 
-
-Lemma proof_of_check_list_gen_safety_wit_6 : check_list_gen_safety_wit_6.
-Proof. Admitted. 
-
-Lemma proof_of_check_list_gen_safety_wit_7 : check_list_gen_safety_wit_7.
-Proof. Admitted. 
-
-Lemma proof_of_check_list_gen_safety_wit_8 : check_list_gen_safety_wit_8.
-Proof. Admitted. 
-
-Lemma proof_of_check_list_gen_safety_wit_9 : check_list_gen_safety_wit_9.
-Proof. Admitted. 
-
 Lemma proof_of_check_list_gen_partial_solve_wit_1 : check_list_gen_partial_solve_wit_1.
 Proof. Admitted. 
 
@@ -153,6 +145,9 @@ Proof. Admitted.
 Lemma proof_of_check_list_gen_partial_solve_wit_7 : check_list_gen_partial_solve_wit_7.
 Proof. Admitted. 
 
+Lemma proof_of_check_list_gen_partial_solve_wit_8_pure : check_list_gen_partial_solve_wit_8_pure.
+Proof. Admitted. 
+
 Lemma proof_of_check_list_gen_partial_solve_wit_8 : check_list_gen_partial_solve_wit_8.
 Proof. Admitted. 
 
@@ -163,50 +158,5 @@ Lemma proof_of_check_list_gen_partial_solve_wit_10 : check_list_gen_partial_solv
 Proof. Admitted. 
 
 Lemma proof_of_check_list_gen_partial_solve_wit_11 : check_list_gen_partial_solve_wit_11.
-Proof. Admitted. 
-
-Lemma proof_of_thm_apply_safety_wit_1 : thm_apply_safety_wit_1.
-Proof. Admitted. 
-
-Lemma proof_of_thm_apply_safety_wit_2 : thm_apply_safety_wit_2.
-Proof. Admitted. 
-
-Lemma proof_of_thm_apply_safety_wit_3 : thm_apply_safety_wit_3.
-Proof. Admitted. 
-
-Lemma proof_of_thm_apply_safety_wit_4 : thm_apply_safety_wit_4.
-Proof. Admitted. 
-
-Lemma proof_of_thm_apply_safety_wit_5 : thm_apply_safety_wit_5.
-Proof. Admitted. 
-
-Lemma proof_of_thm_apply_safety_wit_6 : thm_apply_safety_wit_6.
-Proof. Admitted. 
-
-Lemma proof_of_thm_apply_partial_solve_wit_1 : thm_apply_partial_solve_wit_1.
-Proof. Admitted. 
-
-Lemma proof_of_thm_apply_partial_solve_wit_2 : thm_apply_partial_solve_wit_2.
-Proof. Admitted. 
-
-Lemma proof_of_thm_apply_partial_solve_wit_3 : thm_apply_partial_solve_wit_3.
-Proof. Admitted. 
-
-Lemma proof_of_thm_apply_partial_solve_wit_4_pure : thm_apply_partial_solve_wit_4_pure.
-Proof. Admitted. 
-
-Lemma proof_of_thm_apply_partial_solve_wit_4 : thm_apply_partial_solve_wit_4.
-Proof. Admitted. 
-
-Lemma proof_of_thm_apply_partial_solve_wit_5 : thm_apply_partial_solve_wit_5.
-Proof. Admitted. 
-
-Lemma proof_of_thm_apply_partial_solve_wit_6_pure : thm_apply_partial_solve_wit_6_pure.
-Proof. Admitted. 
-
-Lemma proof_of_thm_apply_partial_solve_wit_6 : thm_apply_partial_solve_wit_6.
-Proof. Admitted. 
-
-Lemma proof_of_thm_apply_partial_solve_wit_7 : thm_apply_partial_solve_wit_7.
 Proof. Admitted. 
 
